add min/max lemmas for array

src/Init/Data/Array/MinMax.lean
@@ -6,8 +6,9 @@ Authors: Paul Reichert
 module
 
 prelude
-import Init.Data.Array.Bootstrap
-import Init.Data.Array.Lemmas
+public import Init.Data.Array.Bootstrap
+public import Init.Data.Array.Lemmas
+public import Init.Data.Array.DecidableEq
 import Init.Data.List.MinMax
 import Init.Data.List.ToArray
 
@@ -24,7 +25,8 @@ Examples:
 * `#[4].min (by decide) = 4`
 * `#[1, 4, 2, 10, 6].min (by decide) = 1`
 -/
-def min [Min α] (arr : Array α) (h : arr.size > 0) : α :=
+public def min [Min α] (arr : Array α) (h : arr ≠ #[]) : α :=
+  haveI : arr.size > 0 := by simp [Array.size_pos_iff, h]
   arr.foldl Min.min arr[0] (start := 1)
 
 /-! ### min? -/
@@ -37,8 +39,8 @@ Examples:
 * `#[4].min? = some 4`
 * `#[1, 4, 2, 10, 6].min? = some 1`
 -/
-def min? [Min α] (arr : Array α) : Option α :=
-  if h : arr.size > 0 then
+public def min? [Min α] (arr : Array α) : Option α :=
+  if h : arr ≠ #[] then
     some (arr.min h)
   else
     none
@@ -52,7 +54,8 @@ Examples:
 * `#[4].max (by decide) = 4`
 * `#[1, 4, 2, 10, 6].max (by decide) = 10`
 -/
-def max [Max α] (arr : Array α) (h : arr.size > 0) : α :=
+public def max [Max α] (arr : Array α) (h : arr ≠ #[]) : α :=
+  haveI : arr.size > 0 := by simp [Array.size_pos_iff, h]
   arr.foldl Max.max arr[0] (start := 1)
 
 /-! ### max? -/
@@ -65,15 +68,15 @@ Examples:
 * `#[4].max? = some 4`
 * `#[1, 4, 2, 10, 6].max? = some 10`
 -/
-def max? [Max α] (arr : Array α) : Option α :=
-  if h : arr.size > 0 then
+public def max? [Max α] (arr : Array α) : Option α :=
+  if h : arr ≠ #[] then
     some (arr.max h)
   else
     none
 
 /-! ### Compatibility with `List` -/
 
-theorem foldlM_eq_foldlM_extract.aux₀ [Monad m] {f : β → α → m β} {xs : Array α} {s hs i j b} :
+theorem foldlM.loop.normalize_stop [Monad m] {f : β → α → m β} {xs : Array α} {s hs i j b} :
     foldlM.loop f xs s hs i j b = foldlM.loop f xs xs.size (Nat.le_refl _) (Min.min i (s - j)) j b := by
   induction i generalizing j b
   · simp [foldlM.loop]
@@ -93,7 +96,7 @@ theorem foldlM_eq_foldlM_extract.aux₀ [Monad m] {f : β → α → m β} {xs :
         rw [this]
       · rfl
 
-theorem foldlM_eq_foldlM_extract.aux [Monad m]
+theorem foldlM.loop.shift_one [Monad m]
     {f : β → α → m β} {xs : Array α} {i j} {b} :
     foldlM.loop f xs xs.size (Nat.le_refl _) i (j + 1) b = foldlM.loop f (xs.toList.drop 1).toArray (xs.size - 1) (by simp) i j b := by
   induction i generalizing j b
@@ -107,19 +110,19 @@ theorem foldlM_eq_foldlM_extract.aux [Monad m]
       simp [ih]
     · rw [dif_neg (by omega)]
 
-theorem foldlM_eq_foldlM_extract.aux₂ [Monad m]
+theorem foldlM.loop.shift [Monad m]
     {f : β → α → m β} {xs : Array α} {i j} {b} :
     foldlM.loop f xs xs.size (Nat.le_refl _) i j b = foldlM.loop f (xs.toList.drop j).toArray (xs.size - j) (by simp) i 0 b := by
   induction j generalizing xs
   · simp
   · rename_i j ih
-    rw [foldlM_eq_foldlM_extract.aux]
+    rw [shift_one]
     specialize ih (xs := (xs.toList.drop 1).toArray)
     simp only [List.drop_drop, Nat.add_comm 1, List.size_toArray, List.length_drop, Array.length_toList] at ih
     rw [ih]
     congr 1; omega
 
-theorem foldlM_eq_foldlM_extract.aux₃ [Monad m]
+theorem foldlM.loop_eq_foldlM_take [Monad m]
     {f : β → α → m β} {xs : Array α} {i} {b} :
     foldlM.loop f xs xs.size (Nat.le_refl _) i 0 b = (xs.toList.take i).foldlM (init := b) f := by
   conv => lhs; rw [← Array.toArray_toList (xs := xs)]
@@ -137,26 +140,24 @@ theorem foldlM_eq_foldlM_extract.aux₃ [Monad m]
         simp at ih
         rw [← ih]
         clear ih
-        simpa using aux (xs := (x :: xs).toArray) (f := f) (b := b') (i := i) (j := 0)
+        simpa using loop.shift_one (xs := (x :: xs).toArray) (f := f) (b := b') (i := i) (j := 0)
     · simp_all
 
-theorem foldlM_eq_foldlM_extract.aux₄ [Monad m] {f : β → α → m β} {xs : Array α} {i b} :
+theorem foldlM.loop_eq_foldlM_extract [Monad m] {f : β → α → m β} {xs : Array α} {i b} :
     foldlM.loop f xs xs.size (Nat.le_refl _) i j b = (xs.extract j (i + j)).foldlM (init := b) f := by
-  rw [aux₂]
-  have := aux₃ (xs := (xs.toList.drop j).toArray) (f := f) (b := b) (i := i)
+  rw [loop.shift]
+  have := loop_eq_foldlM_take (xs := (xs.toList.drop j).toArray) (f := f) (b := b) (i := i)
   simp only [List.size_toArray, List.length_drop, length_toList] at this
   simp only [this, List.take_drop, Nat.add_comm j, ← Array.foldlM_toList, Array.toList_extract]
   simp
 
-theorem foldlM_eq_foldlM_extract [Monad m] {f : β → α → m β} {xs : Array α} {b} :
+public theorem foldlM_eq_foldlM_extract [Monad m] {f : β → α → m β} {xs : Array α} {b} :
     xs.foldlM (init := b) f (start := start) (stop := stop) =
       (xs.extract start stop).foldlM (init := b) f := by
   simp only [foldlM]
   split
   · rw [dif_pos (by omega)]
-    rw [foldlM_eq_foldlM_extract.aux₀]
-    rw [foldlM_eq_foldlM_extract.aux₄]
-    rw [foldlM_eq_foldlM_extract.aux₄]
+    rw [foldlM.loop.normalize_stop, foldlM.loop_eq_foldlM_extract, foldlM.loop_eq_foldlM_extract]
     simp
     congr 1
     · rw [← Array.toArray_toList (xs := xs)]
@@ -165,9 +166,7 @@ theorem foldlM_eq_foldlM_extract [Monad m] {f : β → α → m β} {xs : Array 
       omega
     · omega
   · simp only [size_extract, Nat.le_refl, ↓reduceDIte, Nat.sub_zero]
-    rw [foldlM_eq_foldlM_extract.aux₄]
-    rw [foldlM_eq_foldlM_extract.aux₀]
-    rw [foldlM_eq_foldlM_extract.aux₄]
+    rw [foldlM.loop_eq_foldlM_extract, foldlM.loop.normalize_stop,  foldlM.loop_eq_foldlM_extract]
     simp
     congr 1
     · rw [← Array.toArray_toList (xs := xs)]
@@ -176,13 +175,13 @@ theorem foldlM_eq_foldlM_extract [Monad m] {f : β → α → m β} {xs : Array 
       omega
     · omega
 
-theorem foldl_eq_foldl_extract {xs : Array α} {f : β → α → β} {init : β} :
+public theorem foldl_eq_foldl_extract {xs : Array α} {f : β → α → β} {init : β} :
     xs.foldl (init := init) (start := start) (stop := stop) f = (xs.extract start stop).foldl (init := init) f := by
   simp only [foldl_eq_foldlM]
   rw [foldlM_eq_foldlM_extract]
 
 @[simp, grind =]
-theorem _root_.List.min_toArray [Min α] {l : List α} {h} :
+public theorem _root_.List.min_toArray [Min α] {l : List α} {h} :
     l.toArray.min h = l.min (by simpa [List.ne_nil_iff_length_pos] using h) := by
   let h' : l ≠ [] := by simpa [List.ne_nil_iff_length_pos] using h
   change l.toArray.min h = l.min h'
@@ -196,7 +195,12 @@ theorem _root_.List.min_toArray [Min α] {l : List α} {h} :
       simp [List.min]
 
 @[simp, grind =]
-theorem _root_.List.min?_toArray [Min α] {l : List α} :
+public theorem min_toList [Min α] {xs : Array α} {h} :
+    xs.toList.min h = xs.min (by simpa [List.ne_nil_iff_length_pos] using h) := by
+  cases xs; simp
+
+@[simp, grind =]
+public theorem _root_.List.min?_toArray [Min α] {l : List α} :
     l.toArray.min? = l.min? := by
   rw [Array.min?]
   split
@@ -204,13 +208,12 @@ theorem _root_.List.min?_toArray [Min α] {l : List α} :
   · simp_all
 
 @[simp, grind =]
-theorem min?_toList [Min α] {xs : Array α} :
+public theorem min?_toList [Min α] {xs : Array α} :
     xs.toList.min? = xs.min? := by
-  rcases xs with ⟨l⟩
-  simp
+  cases xs; simp
 
 @[simp, grind =]
-theorem _root_.List.max_toArray [Max α] {l : List α} {h} :
+public theorem _root_.List.max_toArray [Max α] {l : List α} {h} :
     l.toArray.max h = l.max (by simpa [List.ne_nil_iff_length_pos] using h) := by
   let h' : l ≠ [] := by simpa [List.ne_nil_iff_length_pos] using h
   change l.toArray.max h = l.max h'
@@ -223,8 +226,23 @@ theorem _root_.List.max_toArray [Max α] {l : List α} {h} :
       rw [← Array.foldl_toList, Array.toList_extract, List.extract_eq_drop_take]
       simp [List.max]
 
+@[grind =]
+public theorem _root_.List.max_eq_max_toArray [Max α] {l : List α} {h} :
+    l.max h = l.toArray.max (by simpa [List.ne_nil_iff_length_pos] using h) := by
+  simp
+
 @[simp, grind =]
-theorem _root_.List.max?_toArray [Max α] {l : List α} :
+public theorem max_toList [Max α] {xs : Array α} {h} :
+    xs.toList.max h = xs.max (by simpa [List.ne_nil_iff_length_pos] using h) := by
+  cases xs; simp
+
+@[grind =]
+public theorem max_eq_max_toList [Max α] {xs : Array α} {h} :
+    xs.max h = xs.toList.max (by simpa [List.ne_nil_iff_length_pos] using h) := by
+  simp
+
+@[simp, grind =]
+public theorem _root_.List.max?_toArray [Max α] {l : List α} :
     l.toArray.max? = l.max? := by
   rw [Array.max?]
   split
@@ -232,9 +250,201 @@ theorem _root_.List.max?_toArray [Max α] {l : List α} :
   · simp_all
 
 @[simp, grind =]
-theorem max?_toList [Max α] {xs : Array α} :
+public theorem max?_toList [Max α] {xs : Array α} :
     xs.toList.max? = xs.max? := by
+  cases xs; simp
+
+/-! ### Lemmas about `min?` -/
+
+@[simp] public theorem min?_empty [Min α] : (#[] : Array α).min? = none :=
+  (rfl)
+
+@[simp] public theorem min?_singleton [Min α] {x : α} : #[x].min? = some x :=
+  (rfl)
+
+-- We don't put `@[simp]` on `min?_singleton_append'`,
+-- because the definition in terms of `foldl` is not useful for proofs.
+public theorem min?_singleton_append' [Min α] {xs : Array α} :
+    (#[x] ++ xs).min? = some (xs.foldl Min.min x) := by
+  simp [← min?_toList, toList_append, List.min?]
+
+@[simp] public theorem min?_singleton_append [Min α] [Std.Associative (Min.min : α → α → α)] {xs : Array α} :
+    (#[x] ++ xs).min? = some (xs.min?.elim x (Min.min x)) := by
+  simp [← min?_toList, toList_append, List.min?_cons]
+
+@[simp] public theorem min?_eq_none_iff {xs : Array α} [Min α] : xs.min? = none ↔ xs.isEmpty := by
   rcases xs with ⟨l⟩
   simp
+
+public theorem isSome_min?_of_mem {xs : Array α} [Min α] {a : α} (h : a ∈ xs) :
+    xs.min?.isSome := by
+  rw [← min?_toList]
+  apply List.isSome_min?_of_mem (a := a)
+  simpa
+
+public theorem isSome_min?_of_ne_empty [Min α] (xs : Array α) (h : xs ≠ #[]) : xs.min?.isSome := by
+  rw [← min?_toList]
+  apply List.isSome_min?_of_ne_nil
+  simpa
+
+public theorem min?_mem [Min α] [Std.MinEqOr α] (xs : Array α) (h : xs.min? = some a) : a ∈ xs := by
+  rw [← min?_toList] at h
+  simpa using List.min?_mem h
+
+public theorem le_min?_iff [Min α] [LE α] [Std.LawfulOrderInf α] :
+    {xs : Array α} → xs.min? = some a → ∀ {x}, x ≤ a ↔ ∀ b, b ∈ xs → x ≤ b := by
+  intro xs h x
+  simp only [← min?_toList] at h
+  simpa using List.le_min?_iff h
+
+public theorem min?_eq_some_iff [Min α] [LE α] {xs : Array α} [Std.IsLinearOrder α]
+    [Std.LawfulOrderMin α] : xs.min? = some a ↔ a ∈ xs ∧ ∀ b, b ∈ xs → a ≤ b := by
+  rcases xs with ⟨l⟩
+  simpa using List.min?_eq_some_iff
+
+public theorem min?_replicate [Min α] [Std.IdempotentOp (Min.min : α → α → α)] {n : Nat} {a : α} :
+    (replicate n a).min? = if n = 0 then none else some a := by
+  rw [← List.toArray_replicate, List.min?_toArray, List.min?_replicate]
+
+@[simp] public theorem min?_replicate_of_pos [Min α] [Std.MinEqOr α] {n : Nat} {a : α} (h : 0 < n) :
+    (replicate n a).min? = some a := by
+  simp [min?_replicate, Nat.ne_of_gt h]
+
+public theorem foldl_min [Min α] [Std.IdempotentOp (Min.min : α → α → α)] [Std.Associative (Min.min : α → α → α)]
+    {xs : Array α} {a : α} : xs.foldl (init := a) Min.min = Min.min a (xs.min?.getD a) := by
+  rcases xs with ⟨l⟩
+  simp [List.foldl_min]
+
+/-! ### Lemmas about `max?` -/
+
+@[simp] public theorem max?_empty [Max α] : (#[] : Array α).max? = none :=
+  (rfl)
+
+@[simp] public theorem max?_singleton [Max α] {x : α} : #[x].max? = some x :=
+  (rfl)
+
+-- We don't put `@[simp]` on `max?_singleton_append'`,
+-- because the definition in terms of `foldl` is not useful for proofs.
+public theorem max?_singleton_append' [Max α] {xs : Array α} : (#[x] ++ xs).max? = some (xs.foldl Max.max x) := by
+  simp [← max?_toList, toList_append, List.max?]
+
+@[simp] public theorem max?_singleton_append [Max α] [Std.Associative (Max.max : α → α → α)] {xs : Array α} :
+    (#[x] ++ xs).max? = some (xs.max?.elim x (Max.max x)) := by
+  simp [← max?_toList, toList_append, List.max?_cons]
+
+@[simp] public theorem max?_eq_none_iff {xs : Array α} [Max α] : xs.max? = none ↔ xs.isEmpty := by
+  rcases xs with ⟨l⟩
+  simp
+
+public theorem isSome_max?_of_mem {xs : Array α} [Max α] {a : α} (h : a ∈ xs) :
+    xs.max?.isSome := by
+  rw [← max?_toList]
+  apply List.isSome_max?_of_mem (a := a)
+  simpa
+
+public theorem isSome_max?_of_ne_empty [Max α] (xs : Array α) (h : xs ≠ #[]) : xs.max?.isSome := by
+  rw [← max?_toList]
+  apply List.isSome_max?_of_ne_nil
+  simpa
+
+public theorem max?_mem [Max α] [Std.MaxEqOr α] (xs : Array α) (h : xs.max? = some a) : a ∈ xs := by
+  rw [← max?_toList] at h
+  simpa using List.max?_mem h
+
+public theorem max?_le_iff [Max α] [LE α] [Std.LawfulOrderSup α] :
+    {xs : Array α} → xs.max? = some a → ∀ {x}, a ≤ x ↔ ∀ b, b ∈ xs → b ≤ x := by
+  intro xs h x
+  simp only [← max?_toList] at h
+  simpa using List.max?_le_iff h
+
+public theorem max?_eq_some_iff [Max α] [LE α] {xs : Array α} [Std.IsLinearOrder α]
+    [Std.LawfulOrderMax α] : xs.max? = some a ↔ a ∈ xs ∧ ∀ b, b ∈ xs → b ≤ a := by
+  rcases xs with ⟨l⟩
+  simpa using List.max?_eq_some_iff
+
+public theorem max?_replicate [Max α] [Std.IdempotentOp (Max.max : α → α → α)] {n : Nat} {a : α} :
+    (replicate n a).max? = if n = 0 then none else some a := by
+  rw [← List.toArray_replicate, List.max?_toArray, List.max?_replicate]
+
+@[simp] public theorem max?_replicate_of_pos [Max α] [Std.MaxEqOr α] {n : Nat} {a : α} (h : 0 < n) :
+    (replicate n a).max? = some a := by
+  simp [max?_replicate, Nat.ne_of_gt h]
+
+public theorem foldl_max [Max α] [Std.IdempotentOp (Max.max : α → α → α)] [Std.Associative (Max.max : α → α → α)]
+    {xs : Array α} {a : α} : xs.foldl (init := a) Max.max = Max.max a (xs.max?.getD a) := by
+  rcases xs with ⟨l⟩
+  simp [List.foldl_max]
+
+/-! ### Lemmas about `min` -/
+
+public theorem min?_eq_some_min [Min α] : {xs : Array α} → (h : xs ≠ #[]) →
+    xs.min? = some (xs.min h)
+  | ⟨a::as⟩, _ => by simp [Array.min, Array.min?]
+
+public theorem min_eq_get_min? [Min α] : (xs : Array α) → (h : xs ≠ #[]) →
+    xs.min h = xs.min?.get (xs.isSome_min?_of_ne_empty h)
+  | ⟨a::as⟩, _ => by simp [Array.min, Array.min?]
+
+public theorem min_mem [Min α] [Std.MinEqOr α] {xs : Array α} (h : xs ≠ #[]) : xs.min h ∈ xs :=
+  xs.min?_mem (min?_eq_some_min h)
+
+public theorem min_le_of_mem [Min α] [LE α] [Std.IsLinearOrder α] [Std.LawfulOrderMin α]
+    {xs : Array α} {a : α} (ha : a ∈ xs) :
+    xs.min (ne_empty_of_mem ha) ≤ a :=
+  (Array.min?_eq_some_iff.mp (min?_eq_some_min (ne_empty_of_mem ha))).right a ha
+
+public protected theorem le_min_iff [Min α] [LE α] [Std.LawfulOrderInf α]
+    {xs : Array α} (h : xs ≠ #[]) : ∀ {x}, x ≤ xs.min h ↔ ∀ b, b ∈ xs → x ≤ b :=
+  le_min?_iff (min?_eq_some_min h)
+
+public theorem min_eq_iff [Min α] [LE α] {xs : Array α} [Std.IsLinearOrder α] [Std.LawfulOrderMin α]
+    (h : xs ≠ #[]) : xs.min h = a ↔ a ∈ xs ∧ ∀ b, b ∈ xs → a ≤ b := by
+  simpa [min?_eq_some_min h] using (min?_eq_some_iff (xs := xs))
+
+@[simp] public theorem min_replicate [Min α] [Std.MinEqOr α] {n : Nat} {a : α} (h : (replicate n a) ≠ #[]) :
+    (replicate n a).min h = a := by
+  have n_pos : 0 < n := by simpa [Nat.ne_zero_iff_zero_lt] using h
+  simpa [min?_eq_some_min h] using (min?_replicate_of_pos (a := a) n_pos)
+
+public theorem foldl_min_eq_min [Min α] [Std.IdempotentOp (Min.min : α → α → α)]
+    [Std.Associative (Min.min : α → α → α)] {xs : Array α} (h : xs ≠ #[]) {a : α} :
+    xs.foldl Min.min a = Min.min a (xs.min h) := by
+  simpa [min?_eq_some_min h] using foldl_min (xs := xs)
+
+/-! ### Lemmas about `max` -/
+
+public theorem max?_eq_some_max [Max α] : {xs : Array α} → (h : xs ≠ #[]) →
+    xs.max? = some (xs.max h)
+  | ⟨a::as⟩, _ => by simp [Array.max, Array.max?]
+
+public theorem max_eq_get_max? [Max α] : (xs : Array α) → (h : xs ≠ #[]) →
+    xs.max h = xs.max?.get (xs.isSome_max?_of_ne_empty h)
+  | ⟨a::as⟩, _ => by simp [Array.max, Array.max?]
+
+public theorem max_mem [Max α] [Std.MaxEqOr α] {xs : Array α} (h : xs ≠ #[]) : xs.max h ∈ xs :=
+  xs.max?_mem (max?_eq_some_max h)
+
+public protected theorem max_le_iff [Max α] [LE α] [Std.LawfulOrderSup α]
+    {xs : Array α} (h : xs ≠ #[]) : ∀ {x}, xs.max h ≤ x ↔ ∀ b, b ∈ xs → b ≤ x :=
+  max?_le_iff (max?_eq_some_max h)
+
+public theorem max_eq_iff [Max α] [LE α] {xs : Array α} [Std.IsLinearOrder α] [Std.LawfulOrderMax α]
+    (h : xs ≠ #[]) : xs.max h = a ↔ a ∈ xs ∧ ∀ b, b ∈ xs → b ≤ a := by
+  simpa [max?_eq_some_max h] using (max?_eq_some_iff (xs := xs))
+
+public theorem le_max_of_mem [Max α] [LE α] [Std.IsLinearOrder α] [Std.LawfulOrderMax α]
+    {xs : Array α} {a : α} (ha : a ∈ xs) :
+    a ≤ xs.max (ne_empty_of_mem ha) :=
+  (Array.max?_eq_some_iff.mp (max?_eq_some_max (ne_empty_of_mem ha))).right a ha
+
+@[simp] public theorem max_replicate [Max α] [Std.MaxEqOr α] {n : Nat} {a : α} (h : (replicate n a) ≠ #[]) :
+    (replicate n a).max h = a := by
+  have n_pos : 0 < n := by simpa [Nat.ne_zero_iff_zero_lt] using h
+  simpa [max?_eq_some_max h] using (max?_replicate_of_pos (a := a) n_pos)
+
+public theorem foldl_max_eq_max [Max α] [Std.IdempotentOp (Max.max : α → α → α)]
+    [Std.Associative (Max.max : α → α → α)] {xs : Array α} (h : xs ≠ #[]) {a : α} :
+    xs.foldl Max.max a = Max.max a (xs.max h) := by
+  simpa [max?_eq_some_max h] using foldl_max (xs := xs)
 
 end Array
